Switch attarch model to singular environment

src/AttarchProperties.v
@@ -1,5 +1,5 @@
-Require Import TransitionSystems.
 Require Import Privilege.
+Require Import Env.
 Require Import AttarchTrans.
 
 Require Import Ctl.Ctl.
@@ -9,54 +9,54 @@ Open Scope string_scope.
 Open Scope tprop_scope.
 Open Scope env_scope.
 
-Definition useram_key_secure : tprop attarch_state := <[λ '(l, _),
-    forall Γ l' s c,
-      l = sel4_run (l', Γ) s ->
-      read Γ c "useram_key" good_useram_key -> 
-      c = "useram"
-  ]>.
+Definition useram_key_secure : tprop attarch_state := <[λ '(_, Γ),
+  forall c,
+    read Γ c "useram_key" good_useram_key -> 
+    c = "useram"
+]>.
 
 Definition diverged : tprop attarch_state :=
   <[λ '(l, _), l = attarch_bot]>.
 
 Ltac star_notation := 
   repeat change (clos_refl_trans_n1 _ ?R) with (R^*) in *.
-
-
+  
 Theorem useram_key_never_compromised:
-  attarch_trans @attarch_init_state ⊨ AG useram_key_secure.
+  attarch_trans @attarch_good_init_state ⊨ AG useram_key_secure.
 Proof.
+  tcut (AG <[λ '(_, Γ), forall acc b, Γ "useram_key" = Some (acc, b) ->
+             acc = private "useram"]>).
+  { apply AG_weaken.
+    intros [l Γ].
+    tintro H.
+    tentails! in *.
+    intros * (acc & Hlookup & Hacc).
+    do 2 especialize H; forward H by eassumption.
+    subst.
+    unfold private in Hacc.
+    follows apply refl_string_eq in Hacc. }
   apply star__AG.
   intros * Hstar.
   induct! Hstar; star_notation.
   - follows tentails!.
   - invc H.
-    + tentails!.
-      intros * [=] H'; subst!.
-      follows econtradiction no_lookup_no_read.
-    + tentails!.
-      intros * [=] H'; subst!.
-      follows econtradiction no_lookup_no_read.
-    + invc H.
-      * tentails! in *.
-        intros * [=] H'; subst!.
-        eapply IHHstar.
-       -- reflexivity.
-       -- follows eapply write_unchanged_read'.
-      * tentails! in *.
-        intros * [=] H'; subst!.
-        follows eapply IHHstar.
+    + follows tentails!.
+    + follows tentails!.
+    + invc H;
+      tentails! in *;
+      intros;
+      eapply IHHstar;
+      follows write_unchanged_facts.
     + invc H.
       invc H0.
       tentails! in *.
-      intros * [=] H'; subst!.
-      follows eapply IHHstar.
-    + follows tentails!.
+      intros.
+      destruct H5 as (acc' & curr & Hlookup & Hacc & ->).
+      tedious.
+    + follows tentails! in *.
 Qed.
-(* Print Assumptions useram_key_never_compromised. *)
-
-
-Theorem useram_key_never_compromised':
+      
+(* Theorem useram_key_never_compromised':
   attarch_trans @attarch_init_state ⊨ A[useram_key_secure W diverged].
 Proof.
   apply AW_intro; split.
@@ -94,8 +94,32 @@ Proof.
       follows eapply IH.
     + right.
       follows tentails!.
-Qed.
-(* Print Assumptions useram_key_never_compromised'. *)
+Qed. *)
+
+(* Theorems:
+   1. platam key always secure 
+   2. useram key perfectly secure until release 
+     - This may be trivial since useram doesn't have key until release
+     - Maybe not, if the theorem talks about the internal representation 
+       stored by the useram
+   3. Useram key leak is observed unless malicious component acts, steals, 
+      and repairs before platAM notices
+   4. useram evidence is trustworthy unless malicious actor interferes 
+      and useram interacts before the platform am checks in
+ *)
+
+(* Definition platam_key_secure : tprop attarch_state := <[λ '(l, _),
+    forall Γ l' s c,
+      l = sel4_run (l', Γ) s ->
+      read Γ c "useram_key" good_useram_key -> 
+      c = "useram"
+  ]>. *)
+
+
+(* Doesn't separation of gammas make this difficult to talk about *every* environment?
+   Joining of gammas isn't necessarily at odds with composition. Just need to redefine.
+*)
+
 
 Close Scope tprop_scope.
 Close Scope string_scope.
