src/AttarchTrans.v
@@ -1,5 +1,5 @@
 Require Import Privilege.
-Require Import TransitionSystems.
+Require Import Env.
 
 Require Import Ctl.BinaryRelations.
 Require Import Ctl.Definition.
@@ -38,14 +38,11 @@ Inductive platam_label :=
   | platam_meas_release
   | platam_listen.
 
-(* Definition platam_state := dynamic_state platam_label. *)
-Definition platam_state := platam_label × env.
-Definition platam_init_state : platam_state :=
-  (platam_init,
-   private "platam" ? (
-     "platam_key" ↦ encr_platam_key ;;
-     "useram_key_decr_key" ↦ encr_decr_key
-  )).
+Definition platam_init_env : env :=
+  private "platam" ? (
+    "platam_key" ↦ encr_platam_key ;;
+    "useram_key_decr_key" ↦ encr_decr_key
+  ).
 
 Definition decrypt_platam_key key token : platam_key_t := 
   match (key, token) with 
@@ -59,22 +56,22 @@ Definition decrypt_useram_key_decr_key decr_key platam_key : useram_key_decr_key
   | _ => bad_decr_key
   end.
 
-Inductive platam_trans : relation (platam_state × env) := 
-  | platam_unlock_key : forall Γl Γl' Γg key token,
-      read  Γl "platam" "platam_key" key ->
-      read  Γg "platam" "boot_token" token ->
-      write Γl "platam" "platam_key" (decrypt_platam_key key token) Γl' ->
+Inductive platam_trans : relation (platam_label × env) := 
+  | platam_unlock_key : forall Γ Γ' key token,
+      read  Γ "platam" "platam_key" key ->
+      read  Γ "platam" "boot_token" token ->
+      write Γ "platam" "platam_key" (decrypt_platam_key key token) Γ' ->
       platam_trans 
-        (platam_init, Γl, Γg)
-        (platam_meas_release, Γl', Γg)
-  | platam_measure_release : forall Γl Γg Γg' platam_key decr_key,
-      read  Γg "platam" "good_image" true ->
-      read  Γl "platam" "useram_key_decr_key" decr_key ->
-      read  Γl "platam" "platam_key" platam_key -> 
-      write Γg "platam" "vmm_dataport" (decrypt_useram_key_decr_key decr_key platam_key) Γg' ->
+        (platam_init, Γ)
+        (platam_meas_release, Γ')
+  | platam_measure_release : forall Γ Γ' platam_key decr_key,
+      read  Γ "platam" "good_image" true ->
+      read  Γ "platam" "useram_key_decr_key" decr_key ->
+      read  Γ "platam" "platam_key" platam_key -> 
+      write Γ "platam" "vmm_dataport" (decrypt_useram_key_decr_key decr_key platam_key) Γ' ->
       platam_trans 
-        (platam_meas_release, Γl, Γg)
-        (platam_listen, Γl, Γg').
+        (platam_meas_release, Γ)
+        (platam_listen, Γ').
 
 (* TODO, bad_platam_trans, *)
 
@@ -82,10 +79,8 @@ Inductive useram_label :=
   | useram_wait_key
   | useram_listen.
 
-Definition useram_state := useram_label × env.
-
-Definition useram_init_state : useram_state := 
-  (useram_wait_key, private "useram" ? "useram_key" ↦ encr_useram_key).
+Definition useram_init_env : env := 
+  private "useram" ? "useram_key" ↦ encr_useram_key.
 
 Definition decrypt_useram_key key decr_key : useram_key_t := 
   match (key, decr_key) with 
@@ -93,70 +88,78 @@ Definition decrypt_useram_key key decr_key : useram_key_t :=
   | _ => bad_useram_key
   end.
 
-Inductive useram_trans : relation (useram_state × env) :=
-  | useram_get_key : forall Γl Γl' Γg encr_key decr_key,
-      read  Γl "useram" "useram_key" encr_key ->
-      read  Γg "useram" "vmm_dataport" decr_key ->
-      write Γl "useram" "useram_key" (decrypt_useram_key encr_key decr_key) Γl' ->
+Inductive useram_trans : relation (useram_label × env) :=
+  | useram_get_key : forall Γ Γ' encr_key decr_key,
+      read  Γ "useram" "useram_key" encr_key ->
+      read  Γ "useram" "vmm_dataport" decr_key ->
+      write Γ "useram" "useram_key" (decrypt_useram_key encr_key decr_key) Γ' ->
       useram_trans 
-        (useram_wait_key, Γl, Γg)
-        (useram_listen, Γl', Γg).
+        (useram_wait_key, Γ)
+        (useram_listen, Γ').
 
 Inductive vm_label := 
-  | vm_run : useram_state -> vm_label.
+  | vm_run : useram_label -> vm_label.
 
-Definition vm_state := vm_label.
-
-Definition vm_init_state : vm_state := vm_run useram_init_state.
-
-Inductive vm_trans : relation (vm_state × env) := 
+Inductive vm_trans : relation (vm_label × env) := 
   | useram_step : forall x y Γ Γ',
       useram_trans (x, Γ) (y, Γ') ->
       vm_trans (vm_run x, Γ) (vm_run y, Γ').
 
 Inductive attarch_label :=
   | boot
-  | sel4_run : platam_state -> vm_state -> attarch_label
+  | sel4_run : platam_label -> vm_label -> attarch_label
   | attarch_bot.
 
 Definition attarch_state := attarch_label × env.
-
-Definition attarch_init_state : attarch_state := (boot, allReadOnly ? "good_image" ↦ true).
 
 Inductive attarch_trans : relation attarch_state :=
   | boot_good : forall Γ,
       read Γ "root_of_trust" "good_image" true -> 
       attarch_trans
         (boot, Γ)
-        (sel4_run platam_init_state vm_init_state,
-          allReadOnly ? "boot_token" ↦ good_boot_token;; Γ)
+        (sel4_run platam_init (vm_run useram_wait_key),
+          allReadOnly ? "boot_token" ↦ good_boot_token ;;
+          platam_init_env ;;
+          useram_init_env ;;
+          Γ
+        )
   | boot_bad : forall Γ,
       read Γ "root_of_trust" "good_image" false -> 
       attarch_trans
         (boot, Γ)
-        (sel4_run platam_init_state vm_init_state,
-          allReadOnly ? "boot_token" ↦ bad_boot_token;; Γ)
-  | platam_step : forall x l l' Γl Γl' Γg Γg',
-      platam_trans (l, Γl, Γg) (l', Γl', Γg') ->
+        (sel4_run platam_init (vm_run useram_wait_key),
+          allReadOnly ? "boot_token" ↦ bad_boot_token ;;
+          platam_init_env ;;
+          useram_init_env ;;
+          Γ
+        )
+  | platam_step : forall x l l' Γ Γ',
+      platam_trans (l, Γ) (l', Γ') ->
       attarch_trans 
-        (sel4_run (l, Γl) x, Γg)
-        (sel4_run (l', Γl') x, Γg')
-  | vm_step : forall x l l' Γg Γg',
-      vm_trans (l, Γg) (l', Γg') ->
+        (sel4_run l x, Γ)
+        (sel4_run l' x, Γ')
+  | vm_step : forall x l l' Γ Γ',
+      vm_trans (l, Γ) (l', Γ') ->
       attarch_trans 
-        (sel4_run x l, Γg)
-        (sel4_run x l', Γg')
+        (sel4_run x l, Γ)
+        (sel4_run x l', Γ')
  | attarch_diverge : forall l Γ,
       attarch_trans (l, Γ) (attarch_bot, Γ).
 
+Definition attarch_good_init_state : attarch_state := 
+  (boot, allReadOnly ? "good_image" ↦ true).
+
+Definition attarch_bad_init_state : attarch_state := 
+  (boot, allReadOnly ? "good_image" ↦ false).
 
 Lemma attarch_trans_serial : 
   serial_witness attarch_trans.
 Proof using.
-  unfold serial_witness.
+  follows cbv.
+  (* unfold serial_witness.
   intros [l ?].
   eexists.
-  apply attarch_diverge.
+  apply attarch_diverge. *)
 Defined.
 
 Instance transition__attarch_trans : transition attarch_trans :=
