src/Env.v
@@ -1,0 +1,425 @@
+Require Import Privilege.
+
+Require Import Ctl.BinaryRelations.
+Require Import Glib.Glib.
+
+Open Scope string_scope.
+
+(* Partial mappings of variable names to heterogeneous values paired with access controls *)
+
+
+Definition any : Type := Σ t: Type, t.
+Definition box {t} (x: t) : any := existT (λ x, x) t x.
+
+Definition unbox {A} (b: any) (elim: forall t, t -> A) : A :=
+  elim (projT1 b) (projT2 b).
+
+(* TODO: abstract as a section variable? *)
+Definition var  := string.
+Definition comp := string.
+
+Definition env := var -> option (access × any).
+
+Declare Scope env_scope.
+(* Delimit Scope env_scope with env. *)
+Bind Scope env_scope with env.
+Open Scope env_scope.
+
+
+Definition env_empty: env := λ _, None.
+Notation "•" := env_empty : env_scope.
+
+Definition env_singleton {V} var (acc: access) (v: V): env := λ lookup,
+  if lookup =? var then Some (acc, box v) else None.
+Notation "var ↦ v" := (env_singleton var allAcc v)
+  (at level 55, right associativity) : env_scope.
+
+Definition map_access (Γ: env) (acc: access): env := λ lookup, 
+  match Γ lookup with 
+  | Some (_, v) => Some (acc, v)
+  | None => None
+  end.
+Notation "acc ? Γ" := (map_access Γ acc)
+  (at level 60) : env_scope.
+  (* (at level 60, format "acc ?  Γ") : env_scope. *)
+
+(* First env shadows definitions in second *)
+Definition env_concat (Γ1 Γ2: env) : env := λ lookup,
+  match Γ1 lookup with 
+  | Some v => Some v 
+  | None => Γ2 lookup
+  end.
+Notation "Γ1 ;; Γ2" := (env_concat Γ1 Γ2)
+  (at level 65, right associativity) : env_scope.
+
+Definition read {V} (Γ: env) (c: comp) (name: var) (v: V) : Prop :=
+  exists acc: access, 
+    Γ name = Some (acc, box v) /\
+    acc c p_read.
+
+Definition write {V} (Γ: env) (c: comp) (name: var) (v: V) (Γ': env) : Prop :=
+  exists (acc: access) curr,
+    Γ name = Some (acc, curr) /\ 
+    acc c p_write /\ 
+    Γ' = acc ? name ↦ v ;; Γ.
+
+Definition remove_var (Γ: env) var : env := λ lookup,
+  if lookup =? var then None else Γ lookup.
+
+Lemma map_acc_env_singleton : forall acc x V (v: V),
+  (acc ? x ↦ v) = env_singleton x acc v.
+Proof using.
+  intros *.
+  extensionality y.
+  unfold env_singleton.
+  replace (
+    acc ? (λ lookup, 
+      if lookup =? x
+      then Some (allAcc, box v) 
+      else None))
+  with
+    (λ lookup, 
+      if lookup =? x
+      then Some (acc, box v) 
+      else None
+  ).
+  - reflexivity.
+  - extensionality lookup.
+    unfold map_access.
+    follows destruct (lookup =? x).
+Qed.
+
+Lemma refl_string_eq : forall x y,
+  x =? y ->
+  x = y.
+Proof using.
+  intros * ?.
+  follows destruct (eqb_spec x y).
+Qed.
+
+Theorem concat_assoc : forall Γ1 Γ2 Γ3,
+  (Γ1;; Γ2);; Γ3 = Γ1;; (Γ2;; Γ3).
+Proof using.
+  intros *.
+  extensionality s.
+  cbv.
+  follows destruct (Γ1 s).
+Qed.
+
+Theorem env_singleton_inv : forall acc x y V (v: V) v',
+  (acc ? x ↦ v) y = Some v' ->
+  x = y /\ v' = (acc, box v).
+Proof using.
+  intros * H.
+  rewrite map_acc_env_singleton in H.
+  unfold env_singleton in H.
+  destruct (y =? x) eqn:case; [|discriminate].
+  apply refl_string_eq in case as ->.
+  follows inv H.
+Qed.
+
+Theorem env_prepend_singleton_unchanged : forall (Γ: env) x y acc V (v: V),
+  x <> y ->
+  Γ y = (acc ? x ↦ v ;; Γ) y.
+Proof using.
+  intros * Hneq.
+  unfold env_concat.
+  destruct ((acc ? x ↦ v) y) eqn:case. 
+  - apply env_singleton_inv in case as [-> _].
+    contradiction.
+  - reflexivity.
+Qed.
+
+(* Theorem write_unchanged : forall Γ Γ' x y c V (v: V), *)
+Theorem write_unchanged {Γ Γ' x y c V} {v: V}:
+  write Γ c x v Γ' ->
+  x <> y ->
+  Γ y = Γ' y.
+Proof using.
+  intros * Hwrite Hneq.
+  destruct Hwrite as (acc & curr & ? & ? & ->).
+  follows apply env_prepend_singleton_unchanged.
+Qed.
+
+(* Theorem write_unchanged_read : forall Γ Γ' x y c c' V (v: V) V' (v': V'), *)
+Theorem write_unchanged_read {Γ Γ' x y c c' V V'} {v: V} {v': V'}:
+  x <> y ->
+  write Γ c x v Γ' ->
+  read Γ c' y v' ->
+  read Γ' c' y v'.
+Proof using. 
+  intros Hneq Hwrite Hread.
+  unfold read in *.
+  destruct Hread as (acc & Hlookup & Hacc).
+  exists acc.
+  split.
+  - rewrite <- Hlookup.
+    symmetry.
+    follows eapply write_unchanged.
+  - assumption.
+Qed.
+
+(* Theorem write_unchanged_read' : forall Γ Γ' x y c c' V (v: V) V' (v': V'), *)
+Theorem write_unchanged_read' {Γ Γ' x y c c' V V'} {v: V} {v': V'}:
+  x <> y ->
+  write Γ c x v Γ' ->
+  read Γ' c' y v' ->
+  read Γ c' y v'.
+Proof using. 
+  intros Hneq Hwrite Hread.
+  unfold read in *.
+  destruct Hread as (acc & Hlookup & Hacc).
+  exists acc.
+  split.
+  - rewrite <- Hlookup.
+    follows eapply write_unchanged.
+  - assumption.
+Qed.
+
+Theorem no_lookup_no_read {Γ c x V} {v: V}:
+  Γ x = None -> ~ read Γ c x v.
+Proof using.
+  intros * Heq Hread.
+  destruct Hread as (acc & Heq' & _).
+  rewrite Heq in Heq'.
+  discriminate Heq'.
+Qed.
+
+Theorem wrong_lookup_no_read {Γ acc c x V} {w v: V}:
+  Γ x = Some (acc, box w) ->
+  w <> v ->
+  ~ read Γ c x v.
+Proof using.
+  intros * Heq Hneq (? & Heq' & ?).
+  rewritec Heq' in Heq.
+  follows inject Heq.
+Qed.
+
+Theorem good_lookup_read {Γ acc c x V} {w v: V}:
+  Γ x = Some (acc, box w) ->
+  read Γ c x v ->
+  w = v.
+Proof using.
+  intros * Heq (? & Heq' & ?).
+  rewritec Heq' in Heq.
+  follows inject Heq.
+Qed.
+
+Theorem good_lookup_read_replace {Γ acc c x V} {w v: V}:
+  Γ x = Some (acc, box w) ->
+  read Γ c x v ->
+  read Γ c x w.
+Proof using.
+  intros * Heq Hread.
+  inv Hread as (? & Heq' & ?).
+  rewritec Heq' in Heq.
+  follows inject Heq.
+Qed.
+  
+Corollary wrong_lookup_no_read_single_hyp {Γ c x V} {v: V}:
+  (exists acc (w: V), Γ x = Some (acc, box w) /\ w <> v) ->
+  ~ read Γ c x v.
+Proof using.
+  intros H.
+  repeat destructr H.
+  follows eapply wrong_lookup_no_read.
+Qed.
+
+Theorem read_concat_inv {V}: forall Γ1 Γ2 c x (v: V),
+  read (Γ1 ;; Γ2) c x v ->
+  read Γ1 c x v \/ (Γ1 x = None /\ read Γ2 c x v).
+Proof using.
+  intros * H.
+  unfold read in H.
+  destruct (Γ1 x) eqn:case; [left|right].
+  - destruct H as (acc & lookup & H).
+    unfold env_concat in lookup.
+    follows rewrite case in lookup.
+  - destruct H as (acc & lookup & H).
+    unfold env_concat in lookup.
+    follows rewrite case in lookup.
+Qed. 
+
+Theorem read_concat_inv_l {V Γ1 Γ2 c x l} {v: V}:
+  Γ1 x = Some l ->
+  read (Γ1 ;; Γ2) c x v ->
+  read Γ1 c x v.
+Proof using.
+  intros * Heq Hread.
+  unfold read, env_concat in Hread.
+  rewrite Heq in Hread.
+  destruct Hread as (acc & [=->] & Hread).
+  tedious.
+Qed.
+
+Theorem read_concat_inv_l_negative {V Γ1 Γ2 c x} {v: V}:
+  Γ1 x <> None ->
+  read (Γ1 ;; Γ2) c x v ->
+  read Γ1 c x v.
+Proof using.
+  intros * Hneq Hread.
+  destruct (Γ1 x) eqn:case.
+  - clear Hneq.
+    unfold read, env_concat in Hread.
+    rewrite case in Hread.
+    destruct Hread as (acc & [=->] & Hread).
+    tedious.
+  - follows contradict Hneq.
+Qed.
+
+Theorem read_concat_inv_r {V Γ1 Γ2 c x} {v: V}:
+  Γ1 x = None ->
+  read (Γ1 ;; Γ2) c x v ->
+  read Γ2 c x v.
+Proof using.
+  intros * Heq Hread.
+  unfold read, env_concat in Hread.
+  follows rewrite Heq in Hread.
+Qed. 
+ 
+
+Ltac lookup_read H Heq :=
+  match type of H with 
+  | read ?Γ _ ?x _ =>
+      let lookup := eval cbn in (Γ x) in
+      first [
+        (match lookup with 
+        | Some _ => idtac
+        | None => idtac
+        end)
+      | fail 1 "(" Γ x ") does not reduce to a canonical form"];
+      pose proof (eq_refl : Γ x = lookup) as Heq
+  end.
+
+Ltac clookup Γ x cont :=
+  let lookup := eval cbn in (Γ x) in
+  first [
+    (match lookup with 
+    | Some _ => idtac
+    | None => idtac
+    end)
+  | fail 1 "(" Γ x ") does not reduce to a canonical form"];
+  cont lookup.
+
+Ltac simpl_read H :=
+  match type of H with 
+  | read (?Γ1 ;; ?Γ2) _ ?x _ =>
+      clookup Γ1 x ltac:(fun lookup =>
+        match lookup with
+        | Some ?l => simple apply (read_concat_inv_l (eq_refl : Γ1 x = Some l)) in H
+        | None => simple apply (read_concat_inv_r (eq_refl : Γ1 x = None)) in H
+        end
+      )
+  | read ?Γ _ ?x _ =>
+      clookup Γ x ltac:(fun lookup =>
+        let Heq := fresh "Heq" in
+        pose proof (eq_refl : Γ x = lookup) as Heq;
+        match lookup with 
+        | Some (_, box _) =>
+            (* This branch should also add to the environment that the reading 
+               component obeys the access rule we found *)
+            let veq := fresh in 
+            let veq_term := constr:(good_lookup_read Heq H) in
+            lazymatch type of veq_term with 
+            | ?x = ?x => fail
+            | _ => idtac
+            end;
+            pose new proof veq_term as veq;
+            try discriminate veq;
+            subst          
+        | None => exact (False_rect _ (no_lookup_no_read Heq H))
+        end;
+        try clear Heq
+      )
+  end.
+
+Ltac simpl_reads := repeat find simpl_read.
+
+
+Theorem no_lookup_no_write {Γ c x V} {v: V} {Γ'}:
+  Γ x = None -> ~ write Γ c x v Γ'.
+Proof using.
+  intros * Heq (? & ? & lookup & _).
+  rewrite Heq in lookup.
+  discriminate lookup.
+Qed.
+
+Theorem good_lookup_write {Γ acc c x l V} {v: V} {Γ'}:
+  Γ x = Some (acc, l) ->
+  write Γ c x v Γ' ->
+  Γ' = acc ? x ↦ v;; Γ.
+Proof using.
+  intros * Heq (acc' & curr & lookup & ? & ->).
+  rewritec Heq in lookup.
+  follows inject lookup.
+Qed.
+
+Ltac simpl_write H :=
+  match type of H with 
+  | write ?Γ _ ?x _ ?Γ' =>
+      clookup Γ x ltac:(fun lookup =>
+        let Heq := fresh "Heq" in
+        pose proof (eq_refl : Γ x = lookup) as Heq;
+        match lookup with 
+        | Some (_, _) => 
+            let Γeq := fresh in 
+            let Γeq_term := constr:(good_lookup_write Heq H) in
+            lazymatch type of Γeq_term with 
+            | ?x = ?x => fail
+            | _ => idtac
+            end;
+            pose new proof Γeq_term as Γeq;
+            try discriminate Γeq;
+            subst
+        | None => exact (False_rect _ (no_lookup_no_write Heq H))
+        end;
+        try clear Heq
+      )
+  end.
+
+Ltac simpl_writes := repeat find simpl_write.
+
+Ltac write_unchanged_facts :=
+  repeat match goal with 
+  | Hwrite : write ?Γ _ ?x _ ?Γ' |- _ =>
+      repeat match goal with 
+      | Hread : read Γ _ ?y _ |- _ =>
+          let Heq := fresh "Heq" in
+          assert (Heq: x <> y) by discriminate;
+          pose new proof (write_unchanged_read Heq Hwrite Hread);
+          try clear Heq
+      | Hread  : read Γ' _ ?y _ |- _ =>
+          let Heq := fresh "Heq" in
+          assert (Heq: x <> y) by discriminate;
+          pose new proof (write_unchanged_read' Heq Hwrite Hread);
+          try clear Heq
+      | lookup : context[Γ ?y] |- _ =>
+          let Heq := fresh "Heq" in
+          assert (Heq: x <> y) by discriminate;
+          pose new proof (write_unchanged Hwrite Heq);
+          try clear Heq
+      | lookup : context[Γ' ?y] |- _ =>
+          let Heq := fresh "Heq" in
+          assert (Heq: x <> y) by discriminate;
+          pose new proof (write_unchanged Hwrite Heq);
+          try clear Heq
+      | |- context[Γ ?y] =>
+          let Heq := fresh "Heq" in
+          assert (Heq: x <> y) by discriminate;
+          pose new proof (write_unchanged Hwrite Heq);
+          try clear Heq
+      | |- context[Γ' ?y] =>
+          let Heq := fresh "Heq" in
+          assert (Heq: x <> y) by discriminate;
+          pose new proof (write_unchanged Hwrite Heq);
+          try clear Heq
+      end
+  end.
+
+Ltac simpl_rws := repeat find (fun H => simpl_read H || simpl_write H).
+
+Tactic Notation "simpl_rws!" := 
+  repeat (simpl_rws || write_unchanged_facts).
+
+Close Scope env_scope.
+Close Scope string_scope.
